Use new Tick to make progress in tickless inline

compiler/backend/proofs/bvl_inlineProofScript.sml
@@ -4,8 +4,87 @@ open preamble
 
 val _ = new_theory"bvl_inlineProof";
 
-val code_rel_def = Define `
-  code_rel (:'ffi) c1 c2 <=>
+(*
+TODO:
+ - rewrite inline implementation in backend/
+ - prove composition: inline_all = remove_ticks o tick_inline_all
+*)
+
+val mk_tick_F_def = Define `
+  mk_tick_F n e = FUNPOW (Tick F) n e : bvl$exp`;
+
+val attach_tick_def = Define `
+  attach_tick n [] = [] /\
+  attach_tick n xs = FRONT xs ++ [mk_tick_F n (LAST xs)]`;
+
+val var_list_def = Define `
+  var_list n [] [] = T /\
+  var_list n (bvl$Var m :: xs) (y::ys) = (m = n /\ var_list (n+1) xs ys) /\
+  var_list _ _ _ = F`
+
+val dest_op_def = Define `
+  dest_op (bvl$Op op xs) args = (if var_list 0 xs args then SOME op else NONE) /\
+  dest_op _ _ = NONE`
+
+val tick_inline_def = tDefine "tick_inline" `
+  (tick_inline cs [] = []) /\
+  (tick_inline cs (x::y::xs) =
+     HD (tick_inline cs [x]) :: tick_inline cs (y::xs)) /\
+  (tick_inline cs [Var v] = [Var v]) /\
+  (tick_inline cs [If x1 x2 x3] =
+     [If (HD (tick_inline cs [x1]))
+         (HD (tick_inline cs [x2]))
+         (HD (tick_inline cs [x3]))]) /\
+  (tick_inline cs [Let xs x2] =
+     [Let (tick_inline cs xs)
+           (HD (tick_inline cs [x2]))]) /\
+  (tick_inline cs [Raise x1] =
+     [Raise (HD (tick_inline cs [x1]))]) /\
+  (tick_inline cs [Handle x1 x2] =
+     [Handle (HD (tick_inline cs [x1]))
+              (HD (tick_inline cs [x2]))]) /\
+  (tick_inline cs [Op op xs] =
+     [Op op (tick_inline cs xs)]) /\
+  (tick_inline cs [Tick b x] =
+     [Tick b (HD (tick_inline cs [x]))]) /\
+  (tick_inline cs [Call ticks dest xs] =
+     case dest of NONE => [Call ticks dest (tick_inline cs xs)] | SOME n =>
+     case lookup n cs of
+     | NONE => [Call ticks dest (tick_inline cs xs)]
+     | SOME (arity,code) =>
+         case dest_op code xs of
+         | NONE => [Let (tick_inline cs xs) (mk_tick (SUC ticks) code)]
+         | SOME op =>
+           (if NULL xs then [mk_tick (SUC ticks) (Op op [])] else
+             [Op op (attach_tick (SUC ticks) (tick_inline cs xs))]))`
+  (WF_REL_TAC `measure (exp1_size o SND)`);
+
+val tick_inline_ind = theorem"tick_inline_ind";
+
+val tick_inline_all_def = Define `
+  (tick_inline_all limit cs [] aux = REVERSE aux) /\
+  (tick_inline_all limit cs ((n,arity,e1)::xs) aux =
+     let e2 = HD (tick_inline cs [e1]) in
+     let cs2 = if must_inline n limit e2 then insert n (arity,e2) cs else cs in
+       tick_inline_all limit cs2 xs ((n,arity,e2)::aux))`;
+
+val tick_compile_prog_def = Define `
+  tick_compile_prog limit prog =
+    if limit = 0 then prog else tick_inline_all limit LN prog []`
+
+val LENGTH_tick_inline = Q.store_thm("LENGTH_tick_inline",
+  `!cs xs. LENGTH (tick_inline cs xs) = LENGTH xs`,
+  recInduct tick_inline_ind \\ REPEAT STRIP_TAC
+  \\ fs [Once tick_inline_def,LET_DEF] \\ rw [] \\ every_case_tac \\ fs []);
+
+val HD_tick_inline = Q.store_thm("HD_tick_inline[simp]",
+  `[HD (tick_inline cs [x])] = tick_inline cs [x]`,
+  `LENGTH (tick_inline cs [x]) = LENGTH [x]` by SRW_TAC [] [LENGTH_tick_inline]
+  \\ Cases_on `tick_inline cs [x]` \\ FULL_SIMP_TAC std_ss [LENGTH]
+  \\ Cases_on `t` \\ FULL_SIMP_TAC std_ss [LENGTH,HD] \\ `F` by DECIDE_TAC);
+
+val tick_code_rel_def = Define `
+  tick_code_rel (:'ffi) c1 c2 <=>
     !n arity e1.
       lookup n c1 = SOME (arity,e1) ==>
       ?e2. lookup n c2 = SOME (arity,e2) /\
@@ -14,15 +93,15 @@ val code_rel_def = Define `
              evaluate ([e1],env,s with code := c1) = (res,t with code := c1) ==>
              evaluate ([e2],env,s with code := c2) = (res,t with code := c2)`
 
-val code_rel_refl = Q.store_thm("code_rel_refl",
-  `!c. code_rel (:'ffi) c c`,
-  fs [code_rel_def]);
+val tick_code_rel_refl = Q.store_thm("tick_code_rel_refl",
+  `!c. tick_code_rel (:'ffi) c c`,
+  fs [tick_code_rel_def]);
 
-val code_rel_trans = Q.store_thm("code_rel_trans",
+val tick_code_rel_trans = Q.store_thm("tick_code_rel_trans",
   `!c1 c2 c3.
-      code_rel (:'ffi) c1 c2 /\ code_rel (:'ffi) c2 c3 ==>
-      code_rel (:'ffi) c1 c3`,
-  fs [code_rel_def] \\ rw [] \\ res_tac
+      tick_code_rel (:'ffi) c1 c2 /\ tick_code_rel (:'ffi) c2 c3 ==>
+      tick_code_rel (:'ffi) c1 c3`,
+  fs [tick_code_rel_def] \\ rw [] \\ res_tac
   \\ first_x_assum drule \\ rw [] \\ fs []);
 
 val exp_rel_def = Define `
@@ -77,7 +156,15 @@ val evaluate_code_insert = Q.store_thm("evaluate_code_insert",
     \\ first_x_assum drule
     \\ disch_then drule
     \\ fs [exp_rel_def] \\ rw [])
-  \\ TRY (IF_CASES_TAC \\ fs [] \\ NO_TAC)
+  \\ TRY (IF_CASES_TAC \\ fs [] \\ fs [] \\ NO_TAC)
+  THEN1
+   (IF_CASES_TAC \\ fs [] \\ TRY IF_CASES_TAC \\ fs []
+    \\ Cases_on `evaluate ([x],env,s)` \\ fs []
+    \\ `q <> Rerr (Rabort Rtype_error)` by (rpt strip_tac \\ fs [])
+    \\ fs [] \\ imp_res_tac evaluate_code \\ fs []
+    \\ first_x_assum drule
+    \\ disch_then drule \\ fs []
+    \\ Cases_on `q` \\ fs [] \\ IF_CASES_TAC \\ fs [])
   THEN1
    (Cases_on `evaluate (xs,env,s)` \\ fs []
     \\ `q <> Rerr (Rabort Rtype_error)` by (rpt strip_tac \\ fs [])
@@ -129,11 +216,11 @@ val evaluate_code_insert = Q.store_thm("evaluate_code_insert",
     \\ imp_res_tac evaluate_code \\ fs []
     \\ Cases_on `q` \\ fs [] \\ rveq \\ fs []));
 
-val code_rel_insert = Q.store_thm("code_rel_insert",
+val tick_code_rel_insert = Q.store_thm("tick_code_rel_insert",
   `lookup n c = SOME (arity,e1) /\
     exp_rel (:'ffi) (insert n (arity,e2) c) e1 e2 ==>
-    code_rel (:'ffi) c (insert n (arity,e2) c)`,
-  fs [code_rel_def] \\ rw [lookup_insert] \\ rw [] \\ fs [] \\ rw []
+    tick_code_rel (:'ffi) c (insert n (arity,e2) c)`,
+  fs [tick_code_rel_def] \\ rw [lookup_insert] \\ rw [] \\ fs [] \\ rw []
   \\ TRY (drule evaluate_code_insert \\ fs [] \\ NO_TAC)
   \\ drule evaluate_code_insert \\ fs []
   \\ disch_then drule \\ fs [] \\ rw []
@@ -141,37 +228,143 @@ val code_rel_insert = Q.store_thm("code_rel_insert",
   \\ simp_tac std_ss [exp_rel_def]
   \\ disch_then drule \\ fs []);
 
+val attach_ticks_SNOC = prove(
+  ``attach_tick ticks (ys ++ [y]) = ys ++ [mk_tick_F ticks y]``,
+  Cases_on `ys`
+  \\ fs [attach_tick_def]
+  \\ fs [FRONT_DEF]
+  \\ rewrite_tac [GSYM SNOC_APPEND,FRONT_SNOC]);
+
+val evaluate_mk_ticks_F = prove(
+  ``!ticks r y.
+      evaluate ([mk_tick_F ticks y],env,r) =
+      case evaluate ([y],env,r) of
+      | (Rval v,s1) =>
+           if s1.clock < ticks then
+             (Rerr (Rabort Rtimeout_error),s1 with clock := 0)
+           else (Rval v,dec_clock ticks s1)
+      | res => res``,
+  Induct
+  THEN1 (rw [] \\ fs [mk_tick_F_def] \\ every_case_tac \\ fs [])
+  \\ fs [mk_tick_F_def,FUNPOW]
+  \\ fs [evaluate_def] \\ rw []
+  \\ Cases_on `evaluate ([y],env,r)` \\ fs []
+  \\ Cases_on `q` \\ fs []
+  \\ IF_CASES_TAC \\ fs []
+  THEN1 (fs [state_component_equality])
+  \\ fs [dec_clock_def,ADD1]
+  \\ Cases_on `0 < ticks` \\ fs []);
+
+val evaluate_attach_tick = prove(
+  ``~NULL xs ==>
+    evaluate (attach_tick ticks xs,env,s) =
+    case evaluate (xs,env,s) of
+    | (Rerr v,s1) => (Rerr v,s1)
+    | (Rval v,s1) =>
+         if s1.clock < ticks then
+           (Rerr (Rabort Rtimeout_error),s1 with clock := 0)
+         else (Rval v,dec_clock ticks s1)``,
+  `xs = [] \/ ?y ys. xs = SNOC y ys` by metis_tac [SNOC_CASES]
+  \\ fs [] \\ rveq \\ fs [attach_ticks_SNOC]
+  \\ fs [evaluate_APPEND]
+  \\ TOP_CASE_TAC \\ fs []
+  \\ TOP_CASE_TAC \\ fs [evaluate_mk_ticks_F]
+  \\ rpt (TOP_CASE_TAC \\ fs [])
+  \\ rpt (FULL_CASE_TAC \\ fs [])
+  \\ rveq \\ fs []);
+
+val var_list_IMP_evaluate = prove(
+  ``!a2 a1 l xs s.
+      var_list (LENGTH a1) l xs /\ LENGTH (xs:bvl$exp list) = LENGTH a2 ==>
+      evaluate (l,a1++a2,s) = (Rval a2,s)``,
+  Induct THEN1
+   (fs [APPEND_NIL,var_list_def]
+    \\ Cases_on `l` \\ fs [var_list_def,evaluate_def]
+    \\ Cases_on `h` \\ fs [var_list_def,evaluate_def])
+  \\ Cases_on `xs` \\ fs [LENGTH]
+  \\ Cases_on `l` \\ fs [var_list_def]
+  \\ Cases_on `h'` \\ fs [var_list_def]
+  \\ once_rewrite_tac [evaluate_CONS]
+  \\ fs [evaluate_def,EL_LENGTH_APPEND] \\ rw []
+  \\ first_x_assum (qspec_then `a1 ++ [h']` mp_tac)
+  \\ fs [] \\ rw [] \\ res_tac
+  \\ full_simp_tac std_ss [GSYM APPEND_ASSOC,APPEND] \\ fs []);
+
+val var_list_IMP_evaluate = prove(
+  ``var_list 0 l xs /\ LENGTH (xs:bvl$exp list) = LENGTH a ==>
+    evaluate (l,a,s) = (Rval a,s)``,
+  rw []
+  \\ match_mp_tac (Q.SPECL [`xs`,`[]`] var_list_IMP_evaluate
+       |> SIMP_RULE std_ss [APPEND,LENGTH])
+  \\ asm_exists_tac \\ fs []);
+
 fun split_tac q = Cases_on q \\ Cases_on `q` \\ FULL_SIMP_TAC (srw_ss()) [];
 
-val evaluate_inline = Q.store_thm("evaluate_inline",
+val evaluate_tick_inline = Q.store_thm("evaluate_tick_inline",
   `!cs xs s env.
      subspt cs s.code /\
      FST (evaluate (xs,env,s)) <> Rerr(Rabort Rtype_error) ==>
-     (evaluate (inline cs xs,env,s) = evaluate (xs,env,s))`,
-  recInduct inline_ind \\ reverse (REPEAT STRIP_TAC)
-  \\ POP_ASSUM MP_TAC \\ SIMP_TAC std_ss [Once inline_def,LET_DEF] \\ RES_TAC
+     (evaluate (tick_inline cs xs,env,s) = evaluate (xs,env,s))`,
+  recInduct tick_inline_ind \\ reverse (REPEAT STRIP_TAC)
+  \\ POP_ASSUM MP_TAC \\ SIMP_TAC std_ss [Once tick_inline_def,LET_DEF] \\ RES_TAC
   THEN1
    (Cases_on `dest` \\ fs [] THEN1
-     (ONCE_REWRITE_TAC [evaluate_def] \\ ASM_SIMP_TAC std_ss [HD_inline]
+     (ONCE_REWRITE_TAC [evaluate_def] \\ ASM_SIMP_TAC std_ss [HD_tick_inline]
       \\ Cases_on `evaluate (xs,env,s)` \\ FULL_SIMP_TAC std_ss []
       \\ Cases_on `q` \\ FULL_SIMP_TAC (srw_ss()) [LET_DEF])
     \\ Cases_on `lookup x cs` \\ fs [] THEN1
-     (ONCE_REWRITE_TAC [evaluate_def] \\ ASM_SIMP_TAC std_ss [HD_inline]
+     (ONCE_REWRITE_TAC [evaluate_def] \\ ASM_SIMP_TAC std_ss [HD_tick_inline]
       \\ Cases_on `evaluate (xs,env,s)` \\ FULL_SIMP_TAC std_ss []
       \\ Cases_on `q` \\ FULL_SIMP_TAC (srw_ss()) [LET_DEF])
     \\ rename1 `lookup x cs = SOME args`
     \\ PairCases_on `args` \\ fs []
-    \\ ONCE_REWRITE_TAC [evaluate_def] \\ ASM_SIMP_TAC std_ss [HD_inline]
-    \\ Cases_on `evaluate (xs,env,s)` \\ FULL_SIMP_TAC std_ss []
-    \\ Cases_on `q` \\ FULL_SIMP_TAC (srw_ss()) [LET_DEF]
-    \\ IMP_RES_TAC evaluate_code
-    \\ `lookup x s.code = SOME (args0,args1)` by fs [subspt_def,domain_lookup]
-    \\ fs [find_code_def]
-    \\ IMP_RES_TAC evaluate_IMP_LENGTH \\ fs []
+    \\ Cases_on `dest_op args1 xs` \\ fs []
+    THEN1
+     (ONCE_REWRITE_TAC [evaluate_def] \\ ASM_SIMP_TAC std_ss [HD_tick_inline]
+      \\ Cases_on `evaluate (xs,env,s)` \\ FULL_SIMP_TAC std_ss []
+      \\ Cases_on `q` \\ FULL_SIMP_TAC (srw_ss()) [LET_DEF]
+      \\ IMP_RES_TAC evaluate_code
+      \\ `lookup x s.code = SOME (args0,args1)` by fs [subspt_def,domain_lookup]
+      \\ fs [find_code_def]
+      \\ IMP_RES_TAC evaluate_IMP_LENGTH \\ fs []
+      \\ IF_CASES_TAC \\ fs []
+      \\ SIMP_TAC std_ss [evaluate_mk_tick] \\ SRW_TAC [] [] \\ fs [ADD1]
+      \\ MATCH_MP_TAC evaluate_expand_env \\ FULL_SIMP_TAC std_ss [])
     \\ IF_CASES_TAC \\ fs []
-    \\ SIMP_TAC std_ss [evaluate_mk_tick] \\ SRW_TAC [] [] \\ fs [ADD1]
-    \\ MATCH_MP_TAC evaluate_expand_env \\ FULL_SIMP_TAC std_ss [])
-  \\ ONCE_REWRITE_TAC [evaluate_def] \\ ASM_SIMP_TAC std_ss [HD_inline]
+    \\ fs [evaluate_def]
+    THEN1
+     (Cases_on `xs` \\ fs [evaluate_def]
+      \\ TOP_CASE_TAC \\ fs []
+      \\ rename1 `_ = SOME xx` \\ PairCases_on `xx`
+      \\ fs [evaluate_mk_tick,ADD1]
+      \\ IF_CASES_TAC \\ fs []
+      \\ fs [find_code_def]
+      \\ fs [subspt_lookup]
+      \\ res_tac \\ fs [] \\ rveq
+      \\ Cases_on `args1` \\ fs [dest_op_def] \\ rveq
+      \\ Cases_on `l` \\ fs [var_list_def]
+      \\ fs [evaluate_def] \\ Cases_on `h` \\ fs [var_list_def])
+    \\ `~(NULL (tick_inline cs xs))` by
+      (fs [NULL_LENGTH]
+       \\ full_simp_tac std_ss [GSYM LENGTH_NIL,LENGTH_tick_inline])
+    \\ simp [evaluate_attach_tick]
+    \\ Cases_on `evaluate (xs,env,s)` \\ fs []
+    \\ Cases_on `q` \\ fs []
+    \\ TOP_CASE_TAC \\ fs []
+    \\ TOP_CASE_TAC \\ fs [ADD1]
+    \\ TOP_CASE_TAC \\ fs [find_code_def]
+    \\ Cases_on `lookup x r.code` \\ fs []
+    \\ rename1 `_ = SOME yy` \\ PairCases_on `yy` \\ fs [] \\ rveq
+    \\ fs[subspt_lookup] \\ res_tac \\ fs []
+    \\ drule evaluate_code \\ fs [] \\ rw[] \\ fs [] \\ rveq
+    \\ Cases_on `args1` \\ fs [dest_op_def] \\ rveq
+    \\ fs [evaluate_def]
+    \\ imp_res_tac evaluate_IMP_LENGTH
+    \\ qsuff_tac `evaluate (l,a,dec_clock (ticks + 1) r) =
+                   (Rval a,dec_clock (ticks + 1) r)` THEN1 fs []
+    \\ match_mp_tac var_list_IMP_evaluate \\ fs [])
+  \\ TRY (Cases_on `b`)
+  \\ ONCE_REWRITE_TAC [evaluate_def] \\ ASM_SIMP_TAC std_ss [HD_tick_inline]
   \\ TRY (SRW_TAC [] [] \\ FIRST_X_ASSUM MATCH_MP_TAC
           \\ FULL_SIMP_TAC (srw_ss()) [dec_clock_def] \\ NO_TAC)
   \\ TRY (split_tac `evaluate (xs,env,s)`
@@ -179,43 +372,43 @@ val evaluate_inline = Q.store_thm("evaluate_inline",
   \\ TRY (split_tac `evaluate ([x1],env,s)` \\ SRW_TAC [] []
      \\ IMP_RES_TAC evaluate_code \\ FULL_SIMP_TAC (srw_ss()) []
      \\ Cases_on`e`>>fs[]>>NO_TAC)
-  THEN1 (Cases_on `inline cs (y::xs)` THEN1
-      (`LENGTH (inline cs (y::xs)) = 0` by METIS_TAC [LENGTH]
-       \\ FULL_SIMP_TAC std_ss [LENGTH_inline,LENGTH] \\ `F` by DECIDE_TAC)
-     \\ SIMP_TAC std_ss [Once evaluate_def,HD_inline]
+  THEN (Cases_on `tick_inline cs (y::xs)` THEN1
+      (`LENGTH (tick_inline cs (y::xs)) = 0` by METIS_TAC [LENGTH]
+       \\ FULL_SIMP_TAC std_ss [LENGTH_tick_inline,LENGTH] \\ `F` by DECIDE_TAC)
+     \\ SIMP_TAC std_ss [Once evaluate_def,HD_tick_inline]
      \\ POP_ASSUM (fn th => FULL_SIMP_TAC std_ss [GSYM th])
      \\ split_tac `evaluate ([x],env,s)` \\ split_tac `evaluate (y::xs,env,r)`
      \\ IMP_RES_TAC evaluate_code \\ FULL_SIMP_TAC (srw_ss()) []));
 
-val exp_rel_inline = Q.store_thm("exp_rel_inline",
-  `subspt cs c ==> exp_rel (:'ffi) c e (HD (inline cs [e]))`,
+val exp_rel_tick_inline = Q.store_thm("exp_rel_tick_inline",
+  `subspt cs c ==> exp_rel (:'ffi) c e (HD (tick_inline cs [e]))`,
   fs [exp_rel_def] \\ rw []
   \\ qpat_x_assum `_ = (_,_)` (fn th => assume_tac th THEN
         once_rewrite_tac [GSYM th])
-  \\ match_mp_tac evaluate_inline \\ fs []);
+  \\ match_mp_tac evaluate_tick_inline \\ fs []);
 
-val code_rel_insert_inline = Q.store_thm("code_rel_insert_inline",
+val tick_code_rel_insert_tick_inline = Q.store_thm("tick_code_rel_insert_tick_inline",
   `lookup n c = SOME (arity,e1) /\ subspt cs c /\ ~(n IN domain cs) ==>
-    code_rel (:'ffi) c (insert n (arity,(HD (inline cs [e1]))) c)`,
-  rw [] \\ match_mp_tac code_rel_insert \\ fs []
-  \\ match_mp_tac exp_rel_inline
+    tick_code_rel (:'ffi) c (insert n (arity,(HD (tick_inline cs [e1]))) c)`,
+  rw [] \\ match_mp_tac tick_code_rel_insert \\ fs []
+  \\ match_mp_tac exp_rel_tick_inline
   \\ fs [subspt_def,domain_lookup,PULL_EXISTS,lookup_insert]
   \\ rw [] \\ res_tac \\ fs []);
 
-val code_rel_insert_insert_inline = Q.store_thm("code_rel_insert_insert_inline",
+val tick_code_rel_insert_insert_tick_inline = Q.store_thm("tick_code_rel_insert_insert_tick_inline",
   `subspt cs (insert n (arity,e1) c) /\ ~(n IN domain cs) ==>
-    code_rel (:'ffi) (insert n (arity,e1) c)
-                     (insert n (arity,(HD (inline cs [e1]))) c)`,
-  `insert n (arity,HD (inline cs [e1])) c =
-   insert n (arity,HD (inline cs [e1])) (insert n (arity,e1) c)` by fs [insert_shadow]
+    tick_code_rel (:'ffi) (insert n (arity,e1) c)
+                     (insert n (arity,(HD (tick_inline cs [e1]))) c)`,
+  `insert n (arity,HD (tick_inline cs [e1])) c =
+   insert n (arity,HD (tick_inline cs [e1])) (insert n (arity,e1) c)` by fs [insert_shadow]
   \\ pop_assum (fn th => once_rewrite_tac [th]) \\ rw []
-  \\ match_mp_tac code_rel_insert_inline \\ fs []);
+  \\ match_mp_tac tick_code_rel_insert_tick_inline \\ fs []);
 
-val inline_all_acc = Q.store_thm("inline_all_acc",
+val tick_inline_all_acc = Q.store_thm("tick_inline_all_acc",
   `!xs ys cs limit.
-      inline_all limit cs xs ys = REVERSE ys ++ inline_all limit cs xs []`,
-  Induct \\ fs [inline_all_def] \\ strip_tac \\ PairCases_on `h` \\ fs []
-  \\ once_rewrite_tac [inline_all_def] \\ simp_tac std_ss [LET_THM]
+      tick_inline_all limit cs xs ys = REVERSE ys ++ tick_inline_all limit cs xs []`,
+  Induct \\ fs [tick_inline_all_def] \\ strip_tac \\ PairCases_on `h` \\ fs []
+  \\ once_rewrite_tac [tick_inline_all_def] \\ simp_tac std_ss [LET_THM]
   \\ rpt strip_tac \\ IF_CASES_TAC
   \\ qpat_x_assum `!x._` (fn th => once_rewrite_tac [th]) \\ fs []);
 
@@ -229,18 +422,18 @@ val fromAList_SWAP = Q.prove(
   \\ fs [spt_eq_thm,wf_insert,wf_fromAList]
   \\ rw [lookup_insert]);
 
-val code_rel_rearrange_lemma = Q.store_thm("code_rel_rearrange_lemma",
+val tick_code_rel_rearrange_lemma = Q.store_thm("tick_code_rel_rearrange_lemma",
   `ALL_DISTINCT (FST x::MAP FST xs) /\
     MAP FST zs = MAP FST xs /\
-    code_rel (:'ffi) (fromAList (xs++x::ys)) (fromAList (zs++x::ys)) ==>
-    code_rel (:'ffi) (fromAList (x::(xs++ys))) (fromAList (x::(zs++ys))) `,
+    tick_code_rel (:'ffi) (fromAList (xs++x::ys)) (fromAList (zs++x::ys)) ==>
+    tick_code_rel (:'ffi) (fromAList (x::(xs++ys))) (fromAList (x::(zs++ys))) `,
   metis_tac [fromAList_SWAP,APPEND]);
 
-val MAP_FST_inline_all = Q.store_thm("MAP_FST_inline_all",
-  `!xs cs. MAP FST (inline_all limit cs xs []) = MAP FST xs`,
-  Induct \\ fs [inline_all_def] \\ strip_tac
-  \\ PairCases_on `h` \\ fs [inline_all_def] \\ rw []
-  \\ once_rewrite_tac [inline_all_acc] \\ fs []);
+val MAP_FST_tick_inline_all = Q.store_thm("MAP_FST_tick_inline_all",
+  `!xs cs. MAP FST (tick_inline_all limit cs xs []) = MAP FST xs`,
+  Induct \\ fs [tick_inline_all_def] \\ strip_tac
+  \\ PairCases_on `h` \\ fs [tick_inline_all_def] \\ rw []
+  \\ once_rewrite_tac [tick_inline_all_acc] \\ fs []);
 
 val MEM_IMP_ALOOKUP_SOME = Q.store_thm("MEM_IMP_ALOOKUP_SOME",
   `!xs x y.
@@ -249,24 +442,24 @@ val MEM_IMP_ALOOKUP_SOME = Q.store_thm("MEM_IMP_ALOOKUP_SOME",
   Induct \\ fs [FORALL_PROD] \\ rw []
   \\ res_tac \\ fs [MEM_MAP,FORALL_PROD] \\ rfs []);
 
-val code_rel_inline_all = Q.store_thm("code_rel_inline_all",
+val tick_code_rel_tick_inline_all = Q.store_thm("tick_code_rel_tick_inline_all",
   `!xs ys cs.
       (!x y. lookup x cs = SOME y ==> MEM (x,y) ys /\ !y. ~MEM (x,y) xs) /\
       ALL_DISTINCT (MAP FST (ys ++ xs)) ==>
-      code_rel (:'ffi)
+      tick_code_rel (:'ffi)
         (fromAList (xs ++ ys))
-        (fromAList (inline_all limit cs xs [] ++ ys))`,
-  Induct \\ fs [inline_all_def,code_rel_refl]
+        (fromAList (tick_inline_all limit cs xs [] ++ ys))`,
+  Induct \\ fs [tick_inline_all_def,tick_code_rel_refl]
   \\ strip_tac \\ PairCases_on `h` \\ fs []
-  \\ reverse (rw [inline_all_def])
-  \\ once_rewrite_tac [inline_all_acc] \\ fs []
-  \\ qpat_abbrev_tac `zs = inline_all limit _ xs []`
-  \\ match_mp_tac code_rel_trans
-  \\ qexists_tac `fromAList ((h0,h1,HD (inline cs [h2]))::(xs ++ ys))`
+  \\ reverse (rw [tick_inline_all_def])
+  \\ once_rewrite_tac [tick_inline_all_acc] \\ fs []
+  \\ qpat_abbrev_tac `zs = tick_inline_all limit _ xs []`
+  \\ match_mp_tac tick_code_rel_trans
+  \\ qexists_tac `fromAList ((h0,h1,HD (tick_inline cs [h2]))::(xs ++ ys))`
   \\ rpt strip_tac
   \\ TRY
    (fs [fromAList_def]
-    \\ match_mp_tac code_rel_insert_insert_inline
+    \\ match_mp_tac tick_code_rel_insert_insert_tick_inline
     \\ fs [domain_lookup,subspt_def,PULL_EXISTS,lookup_insert]
     \\ reverse (rpt strip_tac) THEN1 (res_tac \\ fs [])
     \\ IF_CASES_TAC \\ fs [] \\ rveq THEN1 (res_tac \\ fs [])
@@ -274,8 +467,8 @@ val code_rel_inline_all = Q.store_thm("code_rel_inline_all",
     \\ fs [lookup_fromAList]
     \\ match_mp_tac MEM_IMP_ALOOKUP_SOME \\ fs []
     \\ fs [ALL_DISTINCT_APPEND] \\ metis_tac [])
-  \\ match_mp_tac code_rel_rearrange_lemma \\ fs []
-  \\ unabbrev_all_tac \\ fs [MAP_FST_inline_all]
+  \\ match_mp_tac tick_code_rel_rearrange_lemma \\ fs []
+  \\ unabbrev_all_tac \\ fs [MAP_FST_tick_inline_all]
   \\ fs [ALL_DISTINCT_APPEND,ALL_DISTINCT]
   \\ first_x_assum match_mp_tac
   \\ fs [ALL_DISTINCT_APPEND,ALL_DISTINCT]
@@ -286,15 +479,15 @@ val code_rel_inline_all = Q.store_thm("code_rel_inline_all",
   \\ Cases_on `y'` \\ fs [])
   |> Q.SPECL [`xs`,`[]`] |> SIMP_RULE std_ss [APPEND_NIL];
 
-val code_rel_compile_prog = Q.store_thm("code_rel_compile_prog",
+val tick_code_rel_tick_compile_prog = Q.store_thm("tick_code_rel_tick_compile_prog",
   `ALL_DISTINCT (MAP FST prog) ==>
-    code_rel (:'ffi) (fromAList prog) (fromAList (compile_prog limit prog))`,
-  fs [compile_prog_def] \\ rw [code_rel_refl]
-  \\ match_mp_tac code_rel_inline_all \\ fs [lookup_def]);
+    tick_code_rel (:'ffi) (fromAList prog) (fromAList (tick_compile_prog limit prog))`,
+  fs [tick_compile_prog_def] \\ rw [tick_code_rel_refl]
+  \\ match_mp_tac tick_code_rel_tick_inline_all \\ fs [lookup_def]);
 
-val code_rel_IMP_semantics_EQ = Q.store_thm("code_rel_IMP_semantics_EQ",
+val tick_code_rel_IMP_semantics_EQ = Q.store_thm("tick_code_rel_IMP_semantics_EQ",
   `!(ffi:'ffi ffi_state) c1 c2 start.
-      code_rel (:'ffi) c1 c2 /\ semantics ffi c1 start <> Fail ==>
+      tick_code_rel (:'ffi) c1 c2 /\ semantics ffi c1 start <> Fail ==>
       semantics ffi c2 start = semantics ffi c1 start`,
   rewrite_tac [GSYM AND_IMP_INTRO]
   \\ ntac 5 strip_tac \\ simp[bvlSemTheory.semantics_def]
@@ -307,7 +500,7 @@ val code_rel_IMP_semantics_EQ = Q.store_thm("code_rel_IMP_semantics_EQ",
     \\ Cases_on `lookup start c1` \\ fs []
     \\ PairCases_on `x` \\ fs []
     \\ IF_CASES_TAC \\ fs [] \\ rveq
-    \\ strip_tac \\ fs [code_rel_def]
+    \\ strip_tac \\ fs [tick_code_rel_def]
     \\ first_x_assum drule \\ strip_tac \\ fs [LENGTH_NIL]
     \\ IF_CASES_TAC \\ fs []
     \\ qpat_x_assum `!x. _ <> _` (qspec_then `k` mp_tac) \\ fs [] \\ rw []
@@ -325,7 +518,7 @@ val code_rel_IMP_semantics_EQ = Q.store_thm("code_rel_IMP_semantics_EQ",
       \\ fs [dec_clock_def,initial_state_def,bvlSemTheory.state_component_equality])
     \\ fs [])
   \\ simp []
-  \\ qpat_x_assum `code_rel (:'ffi) _ _` kall_tac
+  \\ qpat_x_assum `tick_code_rel (:'ffi) _ _` kall_tac
   \\ DEEP_INTRO_TAC some_intro >> simp[] >>
   DEEP_INTRO_TAC some_intro >> simp[] >>
   full_simp_tac(srw_ss())[UNCURRY,LET_THM] >>
@@ -368,14 +561,14 @@ val code_rel_IMP_semantics_EQ = Q.store_thm("code_rel_IMP_semantics_EQ",
     rev_full_simp_tac(srw_ss())[] >> NO_TAC) >>
   srw_tac[][] >> full_simp_tac(srw_ss())[] >> rev_full_simp_tac(srw_ss())[]);
 
-val compile_prog_semantics = save_thm("compile_prog_semantics",
-  MATCH_MP (code_rel_IMP_semantics_EQ |> REWRITE_RULE [GSYM AND_IMP_INTRO])
-   (code_rel_compile_prog |> UNDISCH) |> SPEC_ALL
+val tick_compile_prog_semantics = save_thm("tick_compile_prog_semantics",
+  MATCH_MP (tick_code_rel_IMP_semantics_EQ |> REWRITE_RULE [GSYM AND_IMP_INTRO])
+   (tick_code_rel_tick_compile_prog |> UNDISCH) |> SPEC_ALL
   |> DISCH_ALL |> REWRITE_RULE [AND_IMP_INTRO]);
 
-val MAP_FST_compile_prog = Q.store_thm("MAP_FST_compile_prog",
-  `MAP FST (bvl_inline$compile_prog limit prog) = MAP FST prog`,
-  fs [bvl_inlineTheory.compile_prog_def] \\ rw [MAP_FST_inline_all]);
+val MAP_FST_tick_compile_prog = Q.store_thm("MAP_FST_tick_compile_prog",
+  `MAP FST (tick_compile_prog limit prog) = MAP FST prog`,
+  fs [tick_compile_prog_def] \\ rw [MAP_FST_tick_inline_all]);
 
 (* removal of ticks *)
 
@@ -397,7 +590,7 @@ val remove_ticks_def = tDefine "remove_ticks" `
              (HD (remove_ticks [x2]))]) /\
   (remove_ticks [Op op xs] =
      [Op op (remove_ticks xs)]) /\
-  (remove_ticks [Tick x] = remove_ticks [x]) /\
+  (remove_ticks [Tick b x] = remove_ticks [x]) /\
   (remove_ticks [Call ticks dest xs] =
      [Call 0 dest (remove_ticks xs)])`
   (WF_REL_TAC `measure exp1_size`);
@@ -573,11 +766,24 @@ val evaluate_remove_ticks = Q.store_thm("evaluate_remove_ticks",
     \\ drule do_app_lemma \\ every_case_tac \\ fs []
     \\ rveq \\ fs [])
   THEN1 (* Tick *)
-   (fs [remove_ticks_def]
+   (Cases_on `b` THEN1
+     (fs [remove_ticks_def]
+      \\ first_x_assum drule \\ fs []
+      \\ disch_then drule \\ strip_tac
+      \\ fs [bvlSemTheory.evaluate_def]
+      \\ qexists_tac `ck + 1` \\ fs [dec_clock_def])
+    \\ fs [remove_ticks_def]
     \\ first_x_assum drule \\ fs []
     \\ disch_then drule \\ strip_tac
+    \\ reverse (Cases_on `res`) \\ fs []
+    THEN1 (qexists_tac `ck` \\ fs []
+           \\ fs [bvlSemTheory.evaluate_def])
+    \\ qexists_tac `ck+1` \\ fs []
     \\ fs [bvlSemTheory.evaluate_def]
-    \\ qexists_tac `ck + 1` \\ fs [dec_clock_def])
+    \\ drule evaluate_add_clock \\ fs []
+    \\ disch_then (qspec_then `1` mp_tac)
+    \\ fs [inc_clock_def,dec_clock_def]
+    \\ fs [state_rel_def,state_component_equality])
   (* Call *)
   \\ fs [remove_ticks_def]
   \\ fs [bvlSemTheory.evaluate_def]
@@ -879,5 +1085,51 @@ val compile_prog_semantics = Q.store_thm ("compile_prog_semantics",
        SND,ADD_SYM])
   \\ fs [IS_PREFIX_APPEND]
   \\ simp [EL_APPEND1]);
+
+(* combined theorems *)
+
+val code_rel_def = Define `
+  code_rel (:'ffi) c1 c2 <=>
+    !n arity e1.
+      lookup n c1 = SOME (arity,e1) ==>
+      ?e2. lookup n c2 = SOME (arity,e2) /\
+           !(s:'ffi bvlSem$state) env res t.
+             LENGTH env = arity /\ res <> Rerr (Rabort Rtype_error) /\
+             evaluate ([e1],env,s with code := c1) = (res,t with code := c1) ==>
+             evaluate ([e2],env,s with code := c2) = (res,t with code := c2)`
+
+val code_rel_compile_prog = Q.store_thm("code_rel_compile_prog",
+  `ALL_DISTINCT (MAP FST prog) ==>
+    code_rel (:'ffi) (fromAList prog) (fromAList (compile_prog limit prog))`,
+  cheat);
+
+val code_rel_IMP_semantics_EQ = Q.store_thm("code_rel_IMP_semantics_EQ",
+  `!(ffi:'ffi ffi_state) c1 c2 start.
+      code_rel (:'ffi) c1 c2 /\ semantics ffi c1 start <> Fail ==>
+      semantics ffi c2 start = semantics ffi c1 start`,
+  cheat);
+
+val compile_prog_semantics = save_thm("compile_prog_semantics",
+  MATCH_MP (code_rel_IMP_semantics_EQ |> REWRITE_RULE [GSYM AND_IMP_INTRO])
+   (code_rel_compile_prog |> UNDISCH) |> SPEC_ALL
+  |> DISCH_ALL |> REWRITE_RULE [AND_IMP_INTRO]);
+
+val inline_all_acc = Q.store_thm("inline_all_acc",
+  `!xs ys cs limit.
+      inline_all limit cs xs ys = REVERSE ys ++ inline_all limit cs xs []`,
+  Induct \\ fs [inline_all_def] \\ strip_tac \\ PairCases_on `h` \\ fs []
+  \\ once_rewrite_tac [inline_all_def] \\ simp_tac std_ss [LET_THM]
+  \\ rpt strip_tac \\ IF_CASES_TAC
+  \\ qpat_x_assum `!x._` (fn th => once_rewrite_tac [th]) \\ fs []);
+
+val MAP_FST_inline_all = Q.store_thm("MAP_FST_inline_all",
+  `!xs cs. MAP FST (inline_all limit cs xs []) = MAP FST xs`,
+  Induct \\ fs [inline_all_def] \\ strip_tac
+  \\ PairCases_on `h` \\ fs [inline_all_def] \\ rw []
+  \\ once_rewrite_tac [inline_all_acc] \\ fs []);
+
+val MAP_FST_compile_prog = Q.store_thm("MAP_FST_compile_prog",
+  `MAP FST (compile_prog limit prog) = MAP FST prog`,
+  fs [bvl_inlineTheory.compile_prog_def] \\ rw [MAP_FST_inline_all]);
 
 val _ = export_theory();
